add effect tags on st_term for easier erasure at extraction

pulse/src/ocaml/plugin/generated/Pulse_Checker.ml
@@ -256,7 +256,12 @@ let (instantiate_unknown_witnesses :
                                                                =
                                                                ((Pulse_Syntax_Naming.close_st_term'
                                                                    e x
-                                                                   Prims.int_zero).Pulse_Syntax_Base.range2)
+                                                                   Prims.int_zero).Pulse_Syntax_Base.range2);
+                                                             Pulse_Syntax_Base.effect_tag
+                                                               =
+                                                               ((Pulse_Syntax_Naming.close_st_term'
+                                                                   e x
+                                                                   Prims.int_zero).Pulse_Syntax_Base.effect_tag)
                                                            })) new_names
                                              {
                                                Pulse_Syntax_Base.term1 =
@@ -284,11 +289,17 @@ let (instantiate_unknown_witnesses :
                                                                });
                                                           Pulse_Syntax_Base.range2
                                                             =
-                                                            (t.Pulse_Syntax_Base.range2)
+                                                            (t.Pulse_Syntax_Base.range2);
+                                                          Pulse_Syntax_Base.effect_tag
+                                                            =
+                                                            (t.Pulse_Syntax_Base.effect_tag)
                                                         }
                                                     });
                                                Pulse_Syntax_Base.range2 =
-                                                 (t.Pulse_Syntax_Base.range2)
+                                                 (t.Pulse_Syntax_Base.range2);
+                                               Pulse_Syntax_Base.effect_tag =
+                                                 (Pulse_Syntax_Base.as_effect_hint
+                                                    Pulse_Syntax_Base.STT_Ghost)
                                              })))))) uu___)
 let rec (transform_to_unary_intro_exists :
   Pulse_Typing_Env.env ->
@@ -320,7 +331,9 @@ let rec (transform_to_unary_intro_exists :
                            Obj.repr
                              (FStar_Tactics_Effect.lift_div_tac
                                 (fun uu___ ->
-                                   Pulse_Typing.wr
+                                   Pulse_Typing.wtag
+                                     (FStar_Pervasives_Native.Some
+                                        Pulse_Syntax_Base.STT_Ghost)
                                      (Pulse_Syntax_Base.Tm_IntroExists
                                         {
                                           Pulse_Syntax_Base.p5 = t;
@@ -352,8 +365,8 @@ let rec (transform_to_unary_intro_exists :
                                         "Pulse.Checker.fst"
                                         (Prims.of_int (114))
                                         (Prims.of_int (46))
-                                        (Prims.of_int (120))
-                                        (Prims.of_int (32)))))
+                                        (Prims.of_int (121))
+                                        (Prims.of_int (34)))))
                                (FStar_Tactics_Effect.lift_div_tac
                                   (fun uu___ ->
                                      Pulse_Syntax_Naming.subst_term body
@@ -377,15 +390,16 @@ let rec (transform_to_unary_intro_exists :
                                                    "Pulse.Checker.fst"
                                                    (Prims.of_int (118))
                                                    (Prims.of_int (6))
-                                                   (Prims.of_int (120))
-                                                   (Prims.of_int (32)))))
+                                                   (Prims.of_int (121))
+                                                   (Prims.of_int (34)))))
                                           (Obj.magic
                                              (transform_to_unary_intro_exists
                                                 g body1 ws1))
                                           (fun st ->
                                              FStar_Tactics_Effect.lift_div_tac
                                                (fun uu___ ->
-                                                  Pulse_Typing.wr
+                                                  Pulse_Typing.wtag
+                                                    FStar_Pervasives_Native.None
                                                     (Pulse_Syntax_Base.Tm_Bind
                                                        {
                                                          Pulse_Syntax_Base.binder
@@ -396,7 +410,8 @@ let rec (transform_to_unary_intro_exists :
                                                            = st;
                                                          Pulse_Syntax_Base.body1
                                                            =
-                                                           (Pulse_Typing.wr
+                                                           (Pulse_Typing.wtag
+                                                              FStar_Pervasives_Native.None
                                                               (Pulse_Syntax_Base.Tm_IntroExists
                                                                  {
                                                                    Pulse_Syntax_Base.p5
@@ -423,13 +438,13 @@ let rec (check : Pulse_Checker_Base.check_t) =
                 (FStar_Sealed.seal
                    (Obj.magic
                       (FStar_Range.mk_range "Pulse.Checker.fst"
-                         (Prims.of_int (139)) (Prims.of_int (4))
-                         (Prims.of_int (139)) (Prims.of_int (55)))))
+                         (Prims.of_int (140)) (Prims.of_int (4))
+                         (Prims.of_int (140)) (Prims.of_int (55)))))
                 (FStar_Sealed.seal
                    (Obj.magic
                       (FStar_Range.mk_range "Pulse.Checker.fst"
-                         (Prims.of_int (131)) (Prims.of_int (60))
-                         (Prims.of_int (247)) (Prims.of_int (50)))))
+                         (Prims.of_int (132)) (Prims.of_int (60))
+                         (Prims.of_int (248)) (Prims.of_int (50)))))
                 (Obj.magic
                    (Pulse_Checker_Prover_ElimPure.elim_pure g0 pre0 ()))
                 (fun uu___ ->
@@ -443,17 +458,17 @@ let rec (check : Pulse_Checker_Base.check_t) =
                                   (Obj.magic
                                      (FStar_Range.mk_range
                                         "Pulse.Checker.fst"
-                                        (Prims.of_int (141))
+                                        (Prims.of_int (142))
                                         (Prims.of_int (44))
-                                        (Prims.of_int (243))
+                                        (Prims.of_int (244))
                                         (Prims.of_int (48)))))
                                (FStar_Sealed.seal
                                   (Obj.magic
                                      (FStar_Range.mk_range
                                         "Pulse.Checker.fst"
-                                        (Prims.of_int (244))
+                                        (Prims.of_int (245))
                                         (Prims.of_int (4))
-                                        (Prims.of_int (247))
+                                        (Prims.of_int (248))
                                         (Prims.of_int (50)))))
                                (Obj.magic
                                   (FStar_Tactics_Effect.tac_bind
@@ -461,17 +476,17 @@ let rec (check : Pulse_Checker_Base.check_t) =
                                         (Obj.magic
                                            (FStar_Range.mk_range
                                               "Pulse.Checker.fst"
-                                              (Prims.of_int (142))
+                                              (Prims.of_int (143))
                                               (Prims.of_int (12))
-                                              (Prims.of_int (142))
+                                              (Prims.of_int (143))
                                               (Prims.of_int (55)))))
                                      (FStar_Sealed.seal
                                         (Obj.magic
                                            (FStar_Range.mk_range
                                               "Pulse.Checker.fst"
-                                              (Prims.of_int (143))
+                                              (Prims.of_int (144))
                                               (Prims.of_int (4))
-                                              (Prims.of_int (243))
+                                              (Prims.of_int (244))
                                               (Prims.of_int (48)))))
                                      (FStar_Tactics_Effect.lift_div_tac
                                         (fun uu___1 ->
@@ -522,17 +537,17 @@ let rec (check : Pulse_Checker_Base.check_t) =
                                                           (Obj.magic
                                                              (FStar_Range.mk_range
                                                                 "Pulse.Checker.fst"
-                                                                (Prims.of_int (156))
+                                                                (Prims.of_int (157))
                                                                 (Prims.of_int (13))
-                                                                (Prims.of_int (156))
+                                                                (Prims.of_int (157))
                                                                 (Prims.of_int (46)))))
                                                        (FStar_Sealed.seal
                                                           (Obj.magic
                                                              (FStar_Range.mk_range
                                                                 "Pulse.Checker.fst"
-                                                                (Prims.of_int (156))
+                                                                (Prims.of_int (157))
                                                                 (Prims.of_int (6))
-                                                                (Prims.of_int (166))
+                                                                (Prims.of_int (167))
                                                                 (Prims.of_int (57)))))
                                                        (Obj.magic
                                                           (instantiate_unknown_witnesses
@@ -576,17 +591,17 @@ let rec (check : Pulse_Checker_Base.check_t) =
                                                                     (Obj.magic
                                                                     (FStar_Range.mk_range
                                                                     "Pulse.Checker.fst"
-                                                                    (Prims.of_int (165))
+                                                                    (Prims.of_int (166))
                                                                     (Prims.of_int (19))
-                                                                    (Prims.of_int (165))
+                                                                    (Prims.of_int (166))
                                                                     (Prims.of_int (64)))))
                                                                     (FStar_Sealed.seal
                                                                     (Obj.magic
                                                                     (FStar_Range.mk_range
                                                                     "Pulse.Checker.fst"
-                                                                    (Prims.of_int (166))
+                                                                    (Prims.of_int (167))
                                                                     (Prims.of_int (11))
-                                                                    (Prims.of_int (166))
+                                                                    (Prims.of_int (167))
                                                                     (Prims.of_int (56)))))
                                                                     (Obj.magic
                                                                     (transform_to_unary_intro_exists
@@ -632,17 +647,17 @@ let rec (check : Pulse_Checker_Base.check_t) =
                                                           (Obj.magic
                                                              (FStar_Range.mk_range
                                                                 "Pulse.Checker.fst"
-                                                                (Prims.of_int (175))
+                                                                (Prims.of_int (176))
                                                                 (Prims.of_int (8))
-                                                                (Prims.of_int (191))
+                                                                (Prims.of_int (192))
                                                                 (Prims.of_int (97)))))
                                                        (FStar_Sealed.seal
                                                           (Obj.magic
                                                              (FStar_Range.mk_range
                                                                 "Pulse.Checker.fst"
-                                                                (Prims.of_int (192))
+                                                                (Prims.of_int (193))
                                                                 (Prims.of_int (8))
-                                                                (Prims.of_int (195))
+                                                                (Prims.of_int (196))
                                                                 (Prims.of_int (29)))))
                                                        (match (post_if,
                                                                 post_hint)
@@ -680,18 +695,18 @@ let rec (check : Pulse_Checker_Base.check_t) =
                                                                     (Obj.magic
                                                                     (FStar_Range.mk_range
                                                                     "Pulse.Checker.fst"
-                                                                    (Prims.of_int (181))
+                                                                    (Prims.of_int (182))
                                                                     (Prims.of_int (12))
-                                                                    (Prims.of_int (186))
+                                                                    (Prims.of_int (187))
                                                                     (Prims.of_int (37)))))
                                                                     (
                                                                     FStar_Sealed.seal
                                                                     (Obj.magic
                                                                     (FStar_Range.mk_range
                                                                     "Pulse.Checker.fst"
-                                                                    (Prims.of_int (180))
+                                                                    (Prims.of_int (181))
                                                                     (Prims.of_int (10))
-                                                                    (Prims.of_int (186))
+                                                                    (Prims.of_int (187))
                                                                     (Prims.of_int (37)))))
                                                                     (
                                                                     Obj.magic
@@ -700,17 +715,17 @@ let rec (check : Pulse_Checker_Base.check_t) =
                                                                     (Obj.magic
                                                                     (FStar_Range.mk_range
                                                                     "Pulse.Checker.fst"
-                                                                    (Prims.of_int (186))
+                                                                    (Prims.of_int (187))
                                                                     (Prims.of_int (16))
-                                                                    (Prims.of_int (186))
+                                                                    (Prims.of_int (187))
                                                                     (Prims.of_int (36)))))
                                                                     (FStar_Sealed.seal
                                                                     (Obj.magic
                                                                     (FStar_Range.mk_range
                                                                     "Pulse.Checker.fst"
-                                                                    (Prims.of_int (181))
+                                                                    (Prims.of_int (182))
                                                                     (Prims.of_int (12))
-                                                                    (Prims.of_int (186))
+                                                                    (Prims.of_int (187))
                                                                     (Prims.of_int (37)))))
                                                                     (Obj.magic
                                                                     (Pulse_Syntax_Printer.term_to_string
@@ -725,17 +740,17 @@ let rec (check : Pulse_Checker_Base.check_t) =
                                                                     (Obj.magic
                                                                     (FStar_Range.mk_range
                                                                     "Pulse.Checker.fst"
-                                                                    (Prims.of_int (181))
+                                                                    (Prims.of_int (182))
                                                                     (Prims.of_int (12))
-                                                                    (Prims.of_int (186))
+                                                                    (Prims.of_int (187))
                                                                     (Prims.of_int (37)))))
                                                                     (FStar_Sealed.seal
                                                                     (Obj.magic
                                                                     (FStar_Range.mk_range
                                                                     "Pulse.Checker.fst"
-                                                                    (Prims.of_int (181))
+                                                                    (Prims.of_int (182))
                                                                     (Prims.of_int (12))
-                                                                    (Prims.of_int (186))
+                                                                    (Prims.of_int (187))
                                                                     (Prims.of_int (37)))))
                                                                     (Obj.magic
                                                                     (FStar_Tactics_Effect.tac_bind
@@ -743,9 +758,9 @@ let rec (check : Pulse_Checker_Base.check_t) =
                                                                     (Obj.magic
                                                                     (FStar_Range.mk_range
                                                                     "Pulse.Checker.fst"
-                                                                    (Prims.of_int (185))
+                                                                    (Prims.of_int (186))
                                                                     (Prims.of_int (16))
-                                                                    (Prims.of_int (185))
+                                                                    (Prims.of_int (186))
                                                                     (Prims.of_int (58)))))
                                                                     (FStar_Sealed.seal
                                                                     (Obj.magic
@@ -809,17 +824,17 @@ let rec (check : Pulse_Checker_Base.check_t) =
                                                                     (Obj.magic
                                                                     (FStar_Range.mk_range
                                                                     "Pulse.Checker.fst"
-                                                                    (Prims.of_int (194))
+                                                                    (Prims.of_int (195))
                                                                     (Prims.of_int (8))
-                                                                    (Prims.of_int (194))
+                                                                    (Prims.of_int (195))
                                                                     (Prims.of_int (63)))))
                                                                   (FStar_Sealed.seal
                                                                     (Obj.magic
                                                                     (FStar_Range.mk_range
                                                                     "Pulse.Checker.fst"
-                                                                    (Prims.of_int (192))
+                                                                    (Prims.of_int (193))
                                                                     (Prims.of_int (8))
-                                                                    (Prims.of_int (195))
+                                                                    (Prims.of_int (196))
                                                                     (Prims.of_int (29)))))
                                                                   (Obj.magic
                                                                     (Pulse_Checker_If.check
@@ -866,17 +881,17 @@ let rec (check : Pulse_Checker_Base.check_t) =
                                                           (Obj.magic
                                                              (FStar_Range.mk_range
                                                                 "Pulse.Checker.fst"
-                                                                (Prims.of_int (203))
+                                                                (Prims.of_int (204))
                                                                 (Prims.of_int (8))
-                                                                (Prims.of_int (219))
+                                                                (Prims.of_int (220))
                                                                 (Prims.of_int (97)))))
                                                        (FStar_Sealed.seal
                                                           (Obj.magic
                                                              (FStar_Range.mk_range
                                                                 "Pulse.Checker.fst"
-                                                                (Prims.of_int (220))
+                                                                (Prims.of_int (221))
                                                                 (Prims.of_int (8))
-                                                                (Prims.of_int (223))
+                                                                (Prims.of_int (224))
                                                                 (Prims.of_int (30)))))
                                                        (match (post_match,
                                                                 post_hint)
@@ -914,18 +929,18 @@ let rec (check : Pulse_Checker_Base.check_t) =
                                                                     (Obj.magic
                                                                     (FStar_Range.mk_range
                                                                     "Pulse.Checker.fst"
-                                                                    (Prims.of_int (209))
+                                                                    (Prims.of_int (210))
                                                                     (Prims.of_int (12))
-                                                                    (Prims.of_int (214))
+                                                                    (Prims.of_int (215))
                                                                     (Prims.of_int (37)))))
                                                                     (
                                                                     FStar_Sealed.seal
                                                                     (Obj.magic
                                                                     (FStar_Range.mk_range
                                                                     "Pulse.Checker.fst"
-                                                                    (Prims.of_int (208))
+                                                                    (Prims.of_int (209))
                                                                     (Prims.of_int (10))
-                                                                    (Prims.of_int (214))
+                                                                    (Prims.of_int (215))
                                                                     (Prims.of_int (37)))))
                                                                     (
                                                                     Obj.magic
@@ -934,17 +949,17 @@ let rec (check : Pulse_Checker_Base.check_t) =
                                                                     (Obj.magic
                                                                     (FStar_Range.mk_range
                                                                     "Pulse.Checker.fst"
-                                                                    (Prims.of_int (214))
+                                                                    (Prims.of_int (215))
                                                                     (Prims.of_int (16))
-                                                                    (Prims.of_int (214))
+                                                                    (Prims.of_int (215))
                                                                     (Prims.of_int (36)))))
                                                                     (FStar_Sealed.seal
                                                                     (Obj.magic
                                                                     (FStar_Range.mk_range
                                                                     "Pulse.Checker.fst"
-                                                                    (Prims.of_int (209))
+                                                                    (Prims.of_int (210))
                                                                     (Prims.of_int (12))
-                                                                    (Prims.of_int (214))
+                                                                    (Prims.of_int (215))
                                                                     (Prims.of_int (37)))))
                                                                     (Obj.magic
                                                                     (Pulse_Syntax_Printer.term_to_string
@@ -959,17 +974,17 @@ let rec (check : Pulse_Checker_Base.check_t) =
                                                                     (Obj.magic
                                                                     (FStar_Range.mk_range
                                                                     "Pulse.Checker.fst"
-                                                                    (Prims.of_int (209))
+                                                                    (Prims.of_int (210))
                                                                     (Prims.of_int (12))
-                                                                    (Prims.of_int (214))
+                                                                    (Prims.of_int (215))
                                                                     (Prims.of_int (37)))))
                                                                     (FStar_Sealed.seal
                                                                     (Obj.magic
                                                                     (FStar_Range.mk_range
                                                                     "Pulse.Checker.fst"
-                                                                    (Prims.of_int (209))
+                                                                    (Prims.of_int (210))
                                                                     (Prims.of_int (12))
-                                                                    (Prims.of_int (214))
+                                                                    (Prims.of_int (215))
                                                                     (Prims.of_int (37)))))
                                                                     (Obj.magic
                                                                     (FStar_Tactics_Effect.tac_bind
@@ -977,9 +992,9 @@ let rec (check : Pulse_Checker_Base.check_t) =
                                                                     (Obj.magic
                                                                     (FStar_Range.mk_range
                                                                     "Pulse.Checker.fst"
-                                                                    (Prims.of_int (213))
+                                                                    (Prims.of_int (214))
                                                                     (Prims.of_int (16))
-                                                                    (Prims.of_int (213))
+                                                                    (Prims.of_int (214))
                                                                     (Prims.of_int (58)))))
                                                                     (FStar_Sealed.seal
                                                                     (Obj.magic
@@ -1043,17 +1058,17 @@ let rec (check : Pulse_Checker_Base.check_t) =
                                                                     (Obj.magic
                                                                     (FStar_Range.mk_range
                                                                     "Pulse.Checker.fst"
-                                                                    (Prims.of_int (222))
+                                                                    (Prims.of_int (223))
                                                                     (Prims.of_int (8))
-                                                                    (Prims.of_int (222))
+                                                                    (Prims.of_int (223))
                                                                     (Prims.of_int (65)))))
                                                                   (FStar_Sealed.seal
                                                                     (Obj.magic
                                                                     (FStar_Range.mk_range
                                                                     "Pulse.Checker.fst"
-                                                                    (Prims.of_int (220))
+                                                                    (Prims.of_int (221))
                                                                     (Prims.of_int (8))
-                                                                    (Prims.of_int (223))
+                                                                    (Prims.of_int (224))
                                                                     (Prims.of_int (30)))))
                                                                   (Obj.magic
                                                                     (Pulse_Checker_Match.check
