pulse/src/ocaml/plugin/generated/Pulse_Checker_Prover_ElimExists.ml
@@ -39,7 +39,9 @@ let (mk :
                            FStar_Pervasives_Native.Some
                              (FStar_Pervasives.Mkdtuple4
                                 (nm,
-                                  (Pulse_Typing.wr
+                                  (Pulse_Typing.wtag
+                                     (FStar_Pervasives_Native.Some
+                                        Pulse_Syntax_Base.STT_Ghost)
                                      (Pulse_Syntax_Base.Tm_ElimExists
                                         {
                                           Pulse_Syntax_Base.p4 =
