pulse/src/ocaml/plugin/generated/Pulse_Checker_STApp.ml
@@ -65,7 +65,7 @@ let rec (intro_uvars_for_logical_implicits :
                (Obj.magic
                   (FStar_Range.mk_range "Pulse.Checker.STApp.fst"
                      (Prims.of_int (45)) (Prims.of_int (2))
-                     (Prims.of_int (63)) (Prims.of_int (31)))))
+                     (Prims.of_int (64)) (Prims.of_int (31)))))
             (FStar_Tactics_Effect.lift_div_tac
                (fun uu___ -> Pulse_Syntax_Pure.is_arrow ty))
             (fun uu___ ->
@@ -88,7 +88,7 @@ let rec (intro_uvars_for_logical_implicits :
                                  (FStar_Range.mk_range
                                     "Pulse.Checker.STApp.fst"
                                     (Prims.of_int (47)) (Prims.of_int (37))
-                                    (Prims.of_int (58)) (Prims.of_int (7)))))
+                                    (Prims.of_int (59)) (Prims.of_int (7)))))
                            (FStar_Tactics_Effect.lift_div_tac
                               (fun uu___ ->
                                  Pulse_Typing_Env.fresh
@@ -111,7 +111,7 @@ let rec (intro_uvars_for_logical_implicits :
                                                "Pulse.Checker.STApp.fst"
                                                (Prims.of_int (50))
                                                (Prims.of_int (6))
-                                               (Prims.of_int (57))
+                                               (Prims.of_int (58))
                                                (Prims.of_int (96)))))
                                       (FStar_Tactics_Effect.lift_div_tac
                                          (fun uu___ ->
@@ -149,7 +149,12 @@ let rec (intro_uvars_for_logical_implicits :
                                                                     });
                                                                  Pulse_Syntax_Base.range2
                                                                    =
-                                                                   (t.Pulse_Syntax_Base.range1)
+                                                                   (t.Pulse_Syntax_Base.range1);
+                                                                 Pulse_Syntax_Base.effect_tag
+                                                                   =
+                                                                   (Pulse_Syntax_Base.as_effect_hint
+                                                                    (Pulse_Syntax_Base.ctag_of_comp_st
+                                                                    c_rest))
                                                                }))))
                                             | Pulse_Syntax_Base.C_STAtomic
                                                 (uu___, uu___1) ->
@@ -179,7 +184,12 @@ let rec (intro_uvars_for_logical_implicits :
                                                                     });
                                                                  Pulse_Syntax_Base.range2
                                                                    =
-                                                                   (t.Pulse_Syntax_Base.range1)
+                                                                   (t.Pulse_Syntax_Base.range1);
+                                                                 Pulse_Syntax_Base.effect_tag
+                                                                   =
+                                                                   (Pulse_Syntax_Base.as_effect_hint
+                                                                    (Pulse_Syntax_Base.ctag_of_comp_st
+                                                                    c_rest))
                                                                }))))
                                             | Pulse_Syntax_Base.C_STGhost
                                                 (uu___, uu___1) ->
@@ -209,7 +219,12 @@ let rec (intro_uvars_for_logical_implicits :
                                                                     });
                                                                  Pulse_Syntax_Base.range2
                                                                    =
-                                                                   (t.Pulse_Syntax_Base.range1)
+                                                                   (t.Pulse_Syntax_Base.range1);
+                                                                 Pulse_Syntax_Base.effect_tag
+                                                                   =
+                                                                   (Pulse_Syntax_Base.as_effect_hint
+                                                                    (Pulse_Syntax_Base.ctag_of_comp_st
+                                                                    c_rest))
                                                                }))))
                                             | Pulse_Syntax_Base.C_Tot ty1 ->
                                                 Obj.magic
@@ -230,23 +245,23 @@ let rec (intro_uvars_for_logical_implicits :
                               (Obj.magic
                                  (FStar_Range.mk_range
                                     "Pulse.Checker.STApp.fst"
-                                    (Prims.of_int (61)) (Prims.of_int (6))
-                                    (Prims.of_int (63)) (Prims.of_int (31)))))
+                                    (Prims.of_int (62)) (Prims.of_int (6))
+                                    (Prims.of_int (64)) (Prims.of_int (31)))))
                            (FStar_Sealed.seal
                               (Obj.magic
                                  (FStar_Range.mk_range
                                     "Pulse.Checker.STApp.fst"
-                                    (Prims.of_int (60)) (Prims.of_int (4))
-                                    (Prims.of_int (63)) (Prims.of_int (31)))))
+                                    (Prims.of_int (61)) (Prims.of_int (4))
+                                    (Prims.of_int (64)) (Prims.of_int (31)))))
                            (Obj.magic
                               (FStar_Tactics_Effect.tac_bind
                                  (FStar_Sealed.seal
                                     (Obj.magic
                                        (FStar_Range.mk_range
                                           "Pulse.Checker.STApp.fst"
-                                          (Prims.of_int (63))
+                                          (Prims.of_int (64))
                                           (Prims.of_int (9))
-                                          (Prims.of_int (63))
+                                          (Prims.of_int (64))
                                           (Prims.of_int (30)))))
                                  (FStar_Sealed.seal
                                     (Obj.magic
@@ -269,7 +284,7 @@ let rec (intro_uvars_for_logical_implicits :
                                    (Pulse_Typing_Env.fail g
                                       FStar_Pervasives_Native.None uu___1))
                                 uu___1))) uu___)
-let (instantaite_implicits :
+let (instantiate_implicits :
   Pulse_Typing_Env.env ->
     Pulse_Syntax_Base.st_term ->
       ((Pulse_Typing_Env.env, Pulse_Typing_Env.env,
@@ -282,12 +297,12 @@ let (instantaite_implicits :
         (FStar_Sealed.seal
            (Obj.magic
               (FStar_Range.mk_range "Pulse.Checker.STApp.fst"
-                 (Prims.of_int (71)) (Prims.of_int (14)) (Prims.of_int (71))
+                 (Prims.of_int (72)) (Prims.of_int (14)) (Prims.of_int (72))
                  (Prims.of_int (21)))))
         (FStar_Sealed.seal
            (Obj.magic
               (FStar_Range.mk_range "Pulse.Checker.STApp.fst"
-                 (Prims.of_int (71)) (Prims.of_int (24)) (Prims.of_int (87))
+                 (Prims.of_int (72)) (Prims.of_int (24)) (Prims.of_int (88))
                  (Prims.of_int (32)))))
         (FStar_Tactics_Effect.lift_div_tac
            (fun uu___ -> t.Pulse_Syntax_Base.range2))
@@ -298,13 +313,13 @@ let (instantaite_implicits :
                    (FStar_Sealed.seal
                       (Obj.magic
                          (FStar_Range.mk_range "Pulse.Checker.STApp.fst"
-                            (Prims.of_int (72)) (Prims.of_int (46))
-                            (Prims.of_int (72)) (Prims.of_int (52)))))
+                            (Prims.of_int (73)) (Prims.of_int (46))
+                            (Prims.of_int (73)) (Prims.of_int (52)))))
                    (FStar_Sealed.seal
                       (Obj.magic
                          (FStar_Range.mk_range "Pulse.Checker.STApp.fst"
-                            (Prims.of_int (71)) (Prims.of_int (24))
-                            (Prims.of_int (87)) (Prims.of_int (32)))))
+                            (Prims.of_int (72)) (Prims.of_int (24))
+                            (Prims.of_int (88)) (Prims.of_int (32)))))
                    (FStar_Tactics_Effect.lift_div_tac
                       (fun uu___ -> t.Pulse_Syntax_Base.term1))
                    (fun uu___ ->
@@ -321,17 +336,17 @@ let (instantaite_implicits :
                                      (Obj.magic
                                         (FStar_Range.mk_range
                                            "Pulse.Checker.STApp.fst"
-                                           (Prims.of_int (73))
+                                           (Prims.of_int (74))
                                            (Prims.of_int (17))
-                                           (Prims.of_int (73))
+                                           (Prims.of_int (74))
                                            (Prims.of_int (41)))))
                                   (FStar_Sealed.seal
                                      (Obj.magic
                                         (FStar_Range.mk_range
                                            "Pulse.Checker.STApp.fst"
-                                           (Prims.of_int (73))
+                                           (Prims.of_int (74))
                                            (Prims.of_int (44))
-                                           (Prims.of_int (87))
+                                           (Prims.of_int (88))
                                            (Prims.of_int (32)))))
                                   (FStar_Tactics_Effect.lift_div_tac
                                      (fun uu___1 ->
@@ -345,17 +360,17 @@ let (instantaite_implicits :
                                                 (Obj.magic
                                                    (FStar_Range.mk_range
                                                       "Pulse.Checker.STApp.fst"
-                                                      (Prims.of_int (74))
+                                                      (Prims.of_int (75))
                                                       (Prims.of_int (14))
-                                                      (Prims.of_int (74))
+                                                      (Prims.of_int (75))
                                                       (Prims.of_int (51)))))
                                              (FStar_Sealed.seal
                                                 (Obj.magic
                                                    (FStar_Range.mk_range
                                                       "Pulse.Checker.STApp.fst"
-                                                      (Prims.of_int (73))
+                                                      (Prims.of_int (74))
                                                       (Prims.of_int (44))
-                                                      (Prims.of_int (87))
+                                                      (Prims.of_int (88))
                                                       (Prims.of_int (32)))))
                                              (Obj.magic
                                                 (Pulse_Checker_Pure.instantiate_term_implicits
@@ -419,7 +434,10 @@ let (instantaite_implicits :
                                                                     });
                                                                     Pulse_Syntax_Base.range2
                                                                     =
-                                                                    (t1.Pulse_Syntax_Base.range1)
+                                                                    (t1.Pulse_Syntax_Base.range1);
+                                                                    Pulse_Syntax_Base.effect_tag
+                                                                    =
+                                                                    Pulse_Syntax_Base.default_effect_hint
                                                                     })))
                                                                   | uu___3 ->
                                                                     Obj.repr
@@ -428,17 +446,17 @@ let (instantaite_implicits :
                                                                     (Obj.magic
                                                                     (FStar_Range.mk_range
                                                                     "Pulse.Checker.STApp.fst"
-                                                                    (Prims.of_int (86))
-                                                                    (Prims.of_int (8))
                                                                     (Prims.of_int (87))
+                                                                    (Prims.of_int (8))
+                                                                    (Prims.of_int (88))
                                                                     (Prims.of_int (32)))))
                                                                     (FStar_Sealed.seal
                                                                     (Obj.magic
                                                                     (FStar_Range.mk_range
                                                                     "Pulse.Checker.STApp.fst"
-                                                                    (Prims.of_int (85))
+                                                                    (Prims.of_int (86))
                                                                     (Prims.of_int (6))
-                                                                    (Prims.of_int (87))
+                                                                    (Prims.of_int (88))
                                                                     (Prims.of_int (32)))))
                                                                     (Obj.magic
                                                                     (FStar_Tactics_Effect.tac_bind
@@ -446,9 +464,9 @@ let (instantaite_implicits :
                                                                     (Obj.magic
                                                                     (FStar_Range.mk_range
                                                                     "Pulse.Checker.STApp.fst"
-                                                                    (Prims.of_int (87))
+                                                                    (Prims.of_int (88))
                                                                     (Prims.of_int (11))
-                                                                    (Prims.of_int (87))
+                                                                    (Prims.of_int (88))
                                                                     (Prims.of_int (31)))))
                                                                     (FStar_Sealed.seal
                                                                     (Obj.magic
@@ -503,13 +521,13 @@ let (check :
                 (FStar_Sealed.seal
                    (Obj.magic
                       (FStar_Range.mk_range "Pulse.Checker.STApp.fst"
-                         (Prims.of_int (99)) (Prims.of_int (11))
-                         (Prims.of_int (99)) (Prims.of_int (43)))))
+                         (Prims.of_int (100)) (Prims.of_int (11))
+                         (Prims.of_int (100)) (Prims.of_int (43)))))
                 (FStar_Sealed.seal
                    (Obj.magic
                       (FStar_Range.mk_range "Pulse.Checker.STApp.fst"
-                         (Prims.of_int (99)) (Prims.of_int (46))
-                         (Prims.of_int (186)) (Prims.of_int (123)))))
+                         (Prims.of_int (100)) (Prims.of_int (46))
+                         (Prims.of_int (187)) (Prims.of_int (123)))))
                 (FStar_Tactics_Effect.lift_div_tac
                    (fun uu___ ->
                       Pulse_Checker_Pure.push_context "st_app"
@@ -522,14 +540,14 @@ let (check :
                               (Obj.magic
                                  (FStar_Range.mk_range
                                     "Pulse.Checker.STApp.fst"
-                                    (Prims.of_int (100)) (Prims.of_int (14))
-                                    (Prims.of_int (100)) (Prims.of_int (21)))))
+                                    (Prims.of_int (101)) (Prims.of_int (14))
+                                    (Prims.of_int (101)) (Prims.of_int (21)))))
                            (FStar_Sealed.seal
                               (Obj.magic
                                  (FStar_Range.mk_range
                                     "Pulse.Checker.STApp.fst"
-                                    (Prims.of_int (100)) (Prims.of_int (24))
-                                    (Prims.of_int (186)) (Prims.of_int (123)))))
+                                    (Prims.of_int (101)) (Prims.of_int (24))
+                                    (Prims.of_int (187)) (Prims.of_int (123)))))
                            (FStar_Tactics_Effect.lift_div_tac
                               (fun uu___ -> t.Pulse_Syntax_Base.range2))
                            (fun uu___ ->
@@ -540,20 +558,20 @@ let (check :
                                          (Obj.magic
                                             (FStar_Range.mk_range
                                                "Pulse.Checker.STApp.fst"
-                                               (Prims.of_int (102))
+                                               (Prims.of_int (103))
                                                (Prims.of_int (24))
-                                               (Prims.of_int (102))
+                                               (Prims.of_int (103))
                                                (Prims.of_int (50)))))
                                       (FStar_Sealed.seal
                                          (Obj.magic
                                             (FStar_Range.mk_range
                                                "Pulse.Checker.STApp.fst"
-                                               (Prims.of_int (100))
+                                               (Prims.of_int (101))
                                                (Prims.of_int (24))
-                                               (Prims.of_int (186))
+                                               (Prims.of_int (187))
                                                (Prims.of_int (123)))))
                                       (Obj.magic
-                                         (instantaite_implicits g01 t))
+                                         (instantiate_implicits g01 t))
                                       (fun uu___ ->
                                          (fun uu___ ->
                                             match uu___ with
@@ -565,17 +583,17 @@ let (check :
                                                         (Obj.magic
                                                            (FStar_Range.mk_range
                                                               "Pulse.Checker.STApp.fst"
-                                                              (Prims.of_int (104))
+                                                              (Prims.of_int (105))
                                                               (Prims.of_int (46))
-                                                              (Prims.of_int (104))
+                                                              (Prims.of_int (105))
                                                               (Prims.of_int (52)))))
                                                      (FStar_Sealed.seal
                                                         (Obj.magic
                                                            (FStar_Range.mk_range
                                                               "Pulse.Checker.STApp.fst"
-                                                              (Prims.of_int (102))
+                                                              (Prims.of_int (103))
                                                               (Prims.of_int (53))
-                                                              (Prims.of_int (186))
+                                                              (Prims.of_int (187))
                                                               (Prims.of_int (123)))))
                                                      (FStar_Tactics_Effect.lift_div_tac
                                                         (fun uu___1 ->
@@ -599,18 +617,18 @@ let (check :
                                                                     (Obj.magic
                                                                     (FStar_Range.mk_range
                                                                     "Pulse.Checker.STApp.fst"
-                                                                    (Prims.of_int (106))
+                                                                    (Prims.of_int (107))
                                                                     (Prims.of_int (45))
-                                                                    (Prims.of_int (106))
+                                                                    (Prims.of_int (107))
                                                                     (Prims.of_int (62)))))
                                                                     (
                                                                     FStar_Sealed.seal
                                                                     (Obj.magic
                                                                     (FStar_Range.mk_range
                                                                     "Pulse.Checker.STApp.fst"
-                                                                    (Prims.of_int (104))
+                                                                    (Prims.of_int (105))
                                                                     (Prims.of_int (55))
-                                                                    (Prims.of_int (186))
+                                                                    (Prims.of_int (187))
                                                                     (Prims.of_int (123)))))
                                                                     (
                                                                     Obj.magic
@@ -635,17 +653,17 @@ let (check :
                                                                     (Obj.magic
                                                                     (FStar_Range.mk_range
                                                                     "Pulse.Checker.STApp.fst"
-                                                                    (Prims.of_int (108))
+                                                                    (Prims.of_int (109))
                                                                     (Prims.of_int (2))
-                                                                    (Prims.of_int (112))
+                                                                    (Prims.of_int (113))
                                                                     (Prims.of_int (43)))))
                                                                     (FStar_Sealed.seal
                                                                     (Obj.magic
                                                                     (FStar_Range.mk_range
                                                                     "Pulse.Checker.STApp.fst"
-                                                                    (Prims.of_int (114))
+                                                                    (Prims.of_int (115))
                                                                     (Prims.of_int (2))
-                                                                    (Prims.of_int (186))
+                                                                    (Prims.of_int (187))
                                                                     (Prims.of_int (123)))))
                                                                     (Obj.magic
                                                                     (debug_log
@@ -657,17 +675,17 @@ let (check :
                                                                     (Obj.magic
                                                                     (FStar_Range.mk_range
                                                                     "Pulse.Checker.STApp.fst"
-                                                                    (Prims.of_int (109))
+                                                                    (Prims.of_int (110))
                                                                     (Prims.of_int (12))
-                                                                    (Prims.of_int (112))
+                                                                    (Prims.of_int (113))
                                                                     (Prims.of_int (42)))))
                                                                     (FStar_Sealed.seal
                                                                     (Obj.magic
                                                                     (FStar_Range.mk_range
                                                                     "Pulse.Checker.STApp.fst"
-                                                                    (Prims.of_int (109))
+                                                                    (Prims.of_int (110))
                                                                     (Prims.of_int (4))
-                                                                    (Prims.of_int (112))
+                                                                    (Prims.of_int (113))
                                                                     (Prims.of_int (42)))))
                                                                     (Obj.magic
                                                                     (FStar_Tactics_Effect.tac_bind
@@ -675,17 +693,17 @@ let (check :
                                                                     (Obj.magic
                                                                     (FStar_Range.mk_range
                                                                     "Pulse.Checker.STApp.fst"
-                                                                    (Prims.of_int (112))
+                                                                    (Prims.of_int (113))
                                                                     (Prims.of_int (15))
-                                                                    (Prims.of_int (112))
+                                                                    (Prims.of_int (113))
                                                                     (Prims.of_int (41)))))
                                                                     (FStar_Sealed.seal
                                                                     (Obj.magic
                                                                     (FStar_Range.mk_range
                                                                     "Pulse.Checker.STApp.fst"
-                                                                    (Prims.of_int (109))
+                                                                    (Prims.of_int (110))
                                                                     (Prims.of_int (12))
-                                                                    (Prims.of_int (112))
+                                                                    (Prims.of_int (113))
                                                                     (Prims.of_int (42)))))
                                                                     (Obj.magic
                                                                     (Pulse_Syntax_Printer.term_to_string
@@ -700,35 +718,17 @@ let (check :
                                                                     (Obj.magic
                                                                     (FStar_Range.mk_range
                                                                     "Pulse.Checker.STApp.fst"
-                                                                    (Prims.of_int (109))
+                                                                    (Prims.of_int (110))
                                                                     (Prims.of_int (12))
-                                                                    (Prims.of_int (112))
+                                                                    (Prims.of_int (113))
                                                                     (Prims.of_int (42)))))
                                                                     (FStar_Sealed.seal
                                                                     (Obj.magic
                                                                     (FStar_Range.mk_range
                                                                     "Pulse.Checker.STApp.fst"
-                                                                    (Prims.of_int (109))
+                                                                    (Prims.of_int (110))
                                                                     (Prims.of_int (12))
-                                                                    (Prims.of_int (112))
-                                                                    (Prims.of_int (42)))))
-                                                                    (Obj.magic
-                                                                    (FStar_Tactics_Effect.tac_bind
-                                                                    (FStar_Sealed.seal
-                                                                    (Obj.magic
-                                                                    (FStar_Range.mk_range
-                                                                    "Pulse.Checker.STApp.fst"
-                                                                    (Prims.of_int (109))
-                                                                    (Prims.of_int (12))
-                                                                    (Prims.of_int (112))
-                                                                    (Prims.of_int (42)))))
-                                                                    (FStar_Sealed.seal
-                                                                    (Obj.magic
-                                                                    (FStar_Range.mk_range
-                                                                    "Pulse.Checker.STApp.fst"
-                                                                    (Prims.of_int (109))
-                                                                    (Prims.of_int (12))
-                                                                    (Prims.of_int (112))
+                                                                    (Prims.of_int (113))
                                                                     (Prims.of_int (42)))))
                                                                     (Obj.magic
                                                                     (FStar_Tactics_Effect.tac_bind
@@ -737,8 +737,26 @@ let (check :
                                                                     (FStar_Range.mk_range
                                                                     "Pulse.Checker.STApp.fst"
                                                                     (Prims.of_int (110))
+                                                                    (Prims.of_int (12))
+                                                                    (Prims.of_int (113))
+                                                                    (Prims.of_int (42)))))
+                                                                    (FStar_Sealed.seal
+                                                                    (Obj.magic
+                                                                    (FStar_Range.mk_range
+                                                                    "Pulse.Checker.STApp.fst"
+                                                                    (Prims.of_int (110))
+                                                                    (Prims.of_int (12))
+                                                                    (Prims.of_int (113))
+                                                                    (Prims.of_int (42)))))
+                                                                    (Obj.magic
+                                                                    (FStar_Tactics_Effect.tac_bind
+                                                                    (FStar_Sealed.seal
+                                                                    (Obj.magic
+                                                                    (FStar_Range.mk_range
+                                                                    "Pulse.Checker.STApp.fst"
+                                                                    (Prims.of_int (111))
                                                                     (Prims.of_int (15))
-                                                                    (Prims.of_int (110))
+                                                                    (Prims.of_int (111))
                                                                     (Prims.of_int (38)))))
                                                                     (FStar_Sealed.seal
                                                                     (Obj.magic
@@ -818,17 +836,17 @@ let (check :
                                                                     (Obj.magic
                                                                     (FStar_Range.mk_range
                                                                     "Pulse.Checker.STApp.fst"
-                                                                    (Prims.of_int (117))
+                                                                    (Prims.of_int (118))
                                                                     (Prims.of_int (4))
-                                                                    (Prims.of_int (119))
+                                                                    (Prims.of_int (120))
                                                                     (Prims.of_int (46)))))
                                                                     (FStar_Sealed.seal
                                                                     (Obj.magic
                                                                     (FStar_Range.mk_range
                                                                     "Pulse.Checker.STApp.fst"
-                                                                    (Prims.of_int (119))
+                                                                    (Prims.of_int (120))
                                                                     (Prims.of_int (47))
-                                                                    (Prims.of_int (183))
+                                                                    (Prims.of_int (184))
                                                                     (Prims.of_int (39)))))
                                                                     (Obj.magic
                                                                     (debug_log
@@ -840,17 +858,17 @@ let (check :
                                                                     (Obj.magic
                                                                     (FStar_Range.mk_range
                                                                     "Pulse.Checker.STApp.fst"
-                                                                    (Prims.of_int (118))
-                                                                    (Prims.of_int (14))
                                                                     (Prims.of_int (119))
+                                                                    (Prims.of_int (14))
+                                                                    (Prims.of_int (120))
                                                                     (Prims.of_int (45)))))
                                                                     (FStar_Sealed.seal
                                                                     (Obj.magic
                                                                     (FStar_Range.mk_range
                                                                     "Pulse.Checker.STApp.fst"
-                                                                    (Prims.of_int (118))
-                                                                    (Prims.of_int (6))
                                                                     (Prims.of_int (119))
+                                                                    (Prims.of_int (6))
+                                                                    (Prims.of_int (120))
                                                                     (Prims.of_int (45)))))
                                                                     (Obj.magic
                                                                     (FStar_Tactics_Effect.tac_bind
@@ -858,9 +876,9 @@ let (check :
                                                                     (Obj.magic
                                                                     (FStar_Range.mk_range
                                                                     "Pulse.Checker.STApp.fst"
-                                                                    (Prims.of_int (119))
+                                                                    (Prims.of_int (120))
                                                                     (Prims.of_int (17))
-                                                                    (Prims.of_int (119))
+                                                                    (Prims.of_int (120))
                                                                     (Prims.of_int (44)))))
                                                                     (FStar_Sealed.seal
                                                                     (Obj.magic
@@ -901,17 +919,17 @@ let (check :
                                                                     (Obj.magic
                                                                     (FStar_Range.mk_range
                                                                     "Pulse.Checker.STApp.fst"
-                                                                    (Prims.of_int (121))
+                                                                    (Prims.of_int (122))
                                                                     (Prims.of_int (22))
-                                                                    (Prims.of_int (121))
+                                                                    (Prims.of_int (122))
                                                                     (Prims.of_int (41)))))
                                                                     (FStar_Sealed.seal
                                                                     (Obj.magic
                                                                     (FStar_Range.mk_range
                                                                     "Pulse.Checker.STApp.fst"
-                                                                    (Prims.of_int (122))
+                                                                    (Prims.of_int (123))
                                                                     (Prims.of_int (4))
-                                                                    (Prims.of_int (183))
+                                                                    (Prims.of_int (184))
                                                                     (Prims.of_int (39)))))
                                                                     (FStar_Tactics_Effect.lift_div_tac
                                                                     (fun
@@ -929,17 +947,17 @@ let (check :
                                                                     (Obj.magic
                                                                     (FStar_Range.mk_range
                                                                     "Pulse.Checker.STApp.fst"
-                                                                    (Prims.of_int (122))
+                                                                    (Prims.of_int (123))
                                                                     (Prims.of_int (4))
-                                                                    (Prims.of_int (126))
+                                                                    (Prims.of_int (127))
                                                                     (Prims.of_int (38)))))
                                                                     (FStar_Sealed.seal
                                                                     (Obj.magic
                                                                     (FStar_Range.mk_range
                                                                     "Pulse.Checker.STApp.fst"
-                                                                    (Prims.of_int (128))
+                                                                    (Prims.of_int (129))
                                                                     (Prims.of_int (4))
-                                                                    (Prims.of_int (183))
+                                                                    (Prims.of_int (184))
                                                                     (Prims.of_int (39)))))
                                                                     (if
                                                                     (Prims.op_Negation
@@ -956,17 +974,17 @@ let (check :
                                                                     (Obj.magic
                                                                     (FStar_Range.mk_range
                                                                     "Pulse.Checker.STApp.fst"
-                                                                    (Prims.of_int (125))
-                                                                    (Prims.of_int (11))
                                                                     (Prims.of_int (126))
+                                                                    (Prims.of_int (11))
+                                                                    (Prims.of_int (127))
                                                                     (Prims.of_int (38)))))
                                                                     (FStar_Sealed.seal
                                                                     (Obj.magic
                                                                     (FStar_Range.mk_range
                                                                     "Pulse.Checker.STApp.fst"
-                                                                    (Prims.of_int (124))
+                                                                    (Prims.of_int (125))
                                                                     (Prims.of_int (9))
-                                                                    (Prims.of_int (126))
+                                                                    (Prims.of_int (127))
                                                                     (Prims.of_int (38)))))
                                                                     (Obj.magic
                                                                     (FStar_Tactics_Effect.tac_bind
@@ -974,9 +992,9 @@ let (check :
                                                                     (Obj.magic
                                                                     (FStar_Range.mk_range
                                                                     "Pulse.Checker.STApp.fst"
-                                                                    (Prims.of_int (126))
+                                                                    (Prims.of_int (127))
                                                                     (Prims.of_int (14))
-                                                                    (Prims.of_int (126))
+                                                                    (Prims.of_int (127))
                                                                     (Prims.of_int (37)))))
                                                                     (FStar_Sealed.seal
                                                                     (Obj.magic
@@ -1031,17 +1049,17 @@ let (check :
                                                                     (Obj.magic
                                                                     (FStar_Range.mk_range
                                                                     "Pulse.Checker.STApp.fst"
-                                                                    (Prims.of_int (130))
+                                                                    (Prims.of_int (131))
                                                                     (Prims.of_int (20))
-                                                                    (Prims.of_int (130))
+                                                                    (Prims.of_int (131))
                                                                     (Prims.of_int (64)))))
                                                                     (FStar_Sealed.seal
                                                                     (Obj.magic
                                                                     (FStar_Range.mk_range
                                                                     "Pulse.Checker.STApp.fst"
-                                                                    (Prims.of_int (130))
+                                                                    (Prims.of_int (131))
                                                                     (Prims.of_int (67))
-                                                                    (Prims.of_int (178))
+                                                                    (Prims.of_int (179))
                                                                     (Prims.of_int (104)))))
                                                                     (FStar_Tactics_Effect.lift_div_tac
                                                                     (fun
@@ -1063,17 +1081,17 @@ let (check :
                                                                     (Obj.magic
                                                                     (FStar_Range.mk_range
                                                                     "Pulse.Checker.STApp.fst"
-                                                                    (Prims.of_int (131))
+                                                                    (Prims.of_int (132))
                                                                     (Prims.of_int (28))
-                                                                    (Prims.of_int (131))
+                                                                    (Prims.of_int (132))
                                                                     (Prims.of_int (89)))))
                                                                     (FStar_Sealed.seal
                                                                     (Obj.magic
                                                                     (FStar_Range.mk_range
                                                                     "Pulse.Checker.STApp.fst"
-                                                                    (Prims.of_int (130))
+                                                                    (Prims.of_int (131))
                                                                     (Prims.of_int (67))
-                                                                    (Prims.of_int (178))
+                                                                    (Prims.of_int (179))
                                                                     (Prims.of_int (104)))))
                                                                     (Obj.magic
                                                                     (Pulse_Checker_Pure.check_term_with_expected_type_and_effect
@@ -1096,17 +1114,17 @@ let (check :
                                                                     (Obj.magic
                                                                     (FStar_Range.mk_range
                                                                     "Pulse.Checker.STApp.fst"
-                                                                    (Prims.of_int (133))
+                                                                    (Prims.of_int (134))
                                                                     (Prims.of_int (8))
-                                                                    (Prims.of_int (176))
+                                                                    (Prims.of_int (177))
                                                                     (Prims.of_int (108)))))
                                                                     (FStar_Sealed.seal
                                                                     (Obj.magic
                                                                     (FStar_Range.mk_range
                                                                     "Pulse.Checker.STApp.fst"
-                                                                    (Prims.of_int (131))
+                                                                    (Prims.of_int (132))
                                                                     (Prims.of_int (92))
-                                                                    (Prims.of_int (178))
+                                                                    (Prims.of_int (179))
                                                                     (Prims.of_int (104)))))
                                                                     (match comp_typ
                                                                     with
@@ -1132,7 +1150,12 @@ let (check :
                                                                     = arg1
                                                                     });
                                                                     Pulse_Syntax_Base.range2
-                                                                    = range
+                                                                    = range;
+                                                                    Pulse_Syntax_Base.effect_tag
+                                                                    =
+                                                                    (Pulse_Syntax_Base.as_effect_hint
+                                                                    (Pulse_Syntax_Base.ctag_of_comp_st
+                                                                    comp_typ))
                                                                     },
                                                                     (canon_comp
                                                                     (Pulse_Syntax_Naming.open_comp_with
@@ -1141,6 +1164,7 @@ let (check :
                                                                     (canonicalize_st_typing
                                                                     g
                                                                     (Pulse_Typing.wr
+                                                                    comp_typ
                                                                     (Pulse_Syntax_Base.Tm_STApp
                                                                     {
                                                                     Pulse_Syntax_Base.head
@@ -1184,7 +1208,12 @@ let (check :
                                                                     = arg1
                                                                     });
                                                                     Pulse_Syntax_Base.range2
-                                                                    = range
+                                                                    = range;
+                                                                    Pulse_Syntax_Base.effect_tag
+                                                                    =
+                                                                    (Pulse_Syntax_Base.as_effect_hint
+                                                                    (Pulse_Syntax_Base.ctag_of_comp_st
+                                                                    comp_typ))
                                                                     },
                                                                     (canon_comp
                                                                     (Pulse_Syntax_Naming.open_comp_with
@@ -1193,6 +1222,7 @@ let (check :
                                                                     (canonicalize_st_typing
                                                                     g
                                                                     (Pulse_Typing.wr
+                                                                    comp_typ
                                                                     (Pulse_Syntax_Base.Tm_STApp
                                                                     {
                                                                     Pulse_Syntax_Base.head
@@ -1224,17 +1254,17 @@ let (check :
                                                                     (Obj.magic
                                                                     (FStar_Range.mk_range
                                                                     "Pulse.Checker.STApp.fst"
-                                                                    (Prims.of_int (145))
+                                                                    (Prims.of_int (146))
                                                                     (Prims.of_int (18))
-                                                                    (Prims.of_int (145))
+                                                                    (Prims.of_int (146))
                                                                     (Prims.of_int (25)))))
                                                                     (FStar_Sealed.seal
                                                                     (Obj.magic
                                                                     (FStar_Range.mk_range
                                                                     "Pulse.Checker.STApp.fst"
-                                                                    (Prims.of_int (146))
+                                                                    (Prims.of_int (147))
                                                                     (Prims.of_int (10))
-                                                                    (Prims.of_int (173))
+                                                                    (Prims.of_int (174))
                                                                     (Prims.of_int (23)))))
                                                                     (FStar_Tactics_Effect.lift_div_tac
                                                                     (fun
@@ -1250,17 +1280,17 @@ let (check :
                                                                     (Obj.magic
                                                                     (FStar_Range.mk_range
                                                                     "Pulse.Checker.STApp.fst"
-                                                                    (Prims.of_int (146))
+                                                                    (Prims.of_int (147))
                                                                     (Prims.of_int (10))
-                                                                    (Prims.of_int (148))
+                                                                    (Prims.of_int (149))
                                                                     (Prims.of_int (81)))))
                                                                     (FStar_Sealed.seal
                                                                     (Obj.magic
                                                                     (FStar_Range.mk_range
                                                                     "Pulse.Checker.STApp.fst"
-                                                                    (Prims.of_int (148))
+                                                                    (Prims.of_int (149))
                                                                     (Prims.of_int (82))
-                                                                    (Prims.of_int (173))
+                                                                    (Prims.of_int (174))
                                                                     (Prims.of_int (23)))))
                                                                     (if
                                                                     FStar_Set.mem
@@ -1292,17 +1322,17 @@ let (check :
                                                                     (Obj.magic
                                                                     (FStar_Range.mk_range
                                                                     "Pulse.Checker.STApp.fst"
-                                                                    (Prims.of_int (153))
+                                                                    (Prims.of_int (154))
                                                                     (Prims.of_int (26))
-                                                                    (Prims.of_int (163))
+                                                                    (Prims.of_int (164))
                                                                     (Prims.of_int (50)))))
                                                                     (FStar_Sealed.seal
                                                                     (Obj.magic
                                                                     (FStar_Range.mk_range
                                                                     "Pulse.Checker.STApp.fst"
-                                                                    (Prims.of_int (173))
+                                                                    (Prims.of_int (174))
                                                                     (Prims.of_int (10))
-                                                                    (Prims.of_int (173))
+                                                                    (Prims.of_int (174))
                                                                     (Prims.of_int (23)))))
                                                                     (Obj.magic
                                                                     (FStar_Tactics_Effect.tac_bind
@@ -1310,17 +1340,17 @@ let (check :
                                                                     (Obj.magic
                                                                     (FStar_Range.mk_range
                                                                     "Pulse.Checker.STApp.fst"
-                                                                    (Prims.of_int (155))
-                                                                    (Prims.of_int (14))
                                                                     (Prims.of_int (156))
+                                                                    (Prims.of_int (14))
+                                                                    (Prims.of_int (157))
                                                                     (Prims.of_int (71)))))
                                                                     (FStar_Sealed.seal
                                                                     (Obj.magic
                                                                     (FStar_Range.mk_range
                                                                     "Pulse.Checker.STApp.fst"
-                                                                    (Prims.of_int (157))
+                                                                    (Prims.of_int (158))
                                                                     (Prims.of_int (12))
-                                                                    (Prims.of_int (163))
+                                                                    (Prims.of_int (164))
                                                                     (Prims.of_int (50)))))
                                                                     (Obj.magic
                                                                     (Pulse_Checker_Pure.is_non_informative
@@ -1348,17 +1378,17 @@ let (check :
                                                                     (Obj.magic
                                                                     (FStar_Range.mk_range
                                                                     "Pulse.Checker.STApp.fst"
-                                                                    (Prims.of_int (160))
+                                                                    (Prims.of_int (161))
                                                                     (Prims.of_int (16))
-                                                                    (Prims.of_int (160))
+                                                                    (Prims.of_int (161))
                                                                     (Prims.of_int (103)))))
                                                                     (FStar_Sealed.seal
                                                                     (Obj.magic
                                                                     (FStar_Range.mk_range
                                                                     "Pulse.Checker.STApp.fst"
-                                                                    (Prims.of_int (159))
-                                                                    (Prims.of_int (14))
                                                                     (Prims.of_int (160))
+                                                                    (Prims.of_int (14))
+                                                                    (Prims.of_int (161))
                                                                     (Prims.of_int (103)))))
                                                                     (Obj.magic
                                                                     (FStar_Tactics_Effect.tac_bind
@@ -1366,9 +1396,9 @@ let (check :
                                                                     (Obj.magic
                                                                     (FStar_Range.mk_range
                                                                     "Pulse.Checker.STApp.fst"
-                                                                    (Prims.of_int (160))
+                                                                    (Prims.of_int (161))
                                                                     (Prims.of_int (75))
-                                                                    (Prims.of_int (160))
+                                                                    (Prims.of_int (161))
                                                                     (Prims.of_int (102)))))
                                                                     (FStar_Sealed.seal
                                                                     (Obj.magic
@@ -1442,7 +1472,11 @@ let (check :
                                                                     = arg1
                                                                     });
                                                                     Pulse_Syntax_Base.range2
-                                                                    = range
+                                                                    = range;
+                                                                    Pulse_Syntax_Base.effect_tag
+                                                                    =
+                                                                    (Pulse_Syntax_Base.as_effect_hint
+                                                                    Pulse_Syntax_Base.STT_Ghost)
                                                                     },
                                                                     (canon_comp
                                                                     (Pulse_Syntax_Naming.open_comp_with
@@ -1451,6 +1485,7 @@ let (check :
                                                                     (canonicalize_st_typing
                                                                     g
                                                                     (Pulse_Typing.wr
+                                                                    comp_typ
                                                                     (Pulse_Syntax_Base.Tm_STApp
                                                                     {
                                                                     Pulse_Syntax_Base.head
@@ -1499,17 +1534,17 @@ let (check :
                                                                     (Obj.magic
                                                                     (FStar_Range.mk_range
                                                                     "Pulse.Checker.STApp.fst"
-                                                                    (Prims.of_int (178))
+                                                                    (Prims.of_int (179))
                                                                     (Prims.of_int (8))
-                                                                    (Prims.of_int (178))
+                                                                    (Prims.of_int (179))
                                                                     (Prims.of_int (104)))))
                                                                     (FStar_Sealed.seal
                                                                     (Obj.magic
                                                                     (FStar_Range.mk_range
                                                                     "Pulse.Checker.STApp.fst"
-                                                                    (Prims.of_int (178))
+                                                                    (Prims.of_int (179))
                                                                     (Prims.of_int (8))
-                                                                    (Prims.of_int (178))
+                                                                    (Prims.of_int (179))
                                                                     (Prims.of_int (104)))))
                                                                     (FStar_Tactics_Effect.lift_div_tac
                                                                     (fun
@@ -1525,17 +1560,17 @@ let (check :
                                                                     (Obj.magic
                                                                     (FStar_Range.mk_range
                                                                     "Pulse.Checker.STApp.fst"
-                                                                    (Prims.of_int (178))
+                                                                    (Prims.of_int (179))
                                                                     (Prims.of_int (31))
-                                                                    (Prims.of_int (178))
+                                                                    (Prims.of_int (179))
                                                                     (Prims.of_int (86)))))
                                                                     (FStar_Sealed.seal
                                                                     (Obj.magic
                                                                     (FStar_Range.mk_range
                                                                     "Pulse.Checker.STApp.fst"
-                                                                    (Prims.of_int (178))
+                                                                    (Prims.of_int (179))
                                                                     (Prims.of_int (8))
-                                                                    (Prims.of_int (178))
+                                                                    (Prims.of_int (179))
                                                                     (Prims.of_int (104)))))
                                                                     (Obj.magic
                                                                     (Pulse_Checker_Prover.try_frame_pre_uvs
@@ -1565,17 +1600,17 @@ let (check :
                                                                     (Obj.magic
                                                                     (FStar_Range.mk_range
                                                                     "Pulse.Checker.STApp.fst"
-                                                                    (Prims.of_int (180))
+                                                                    (Prims.of_int (181))
                                                                     (Prims.of_int (31))
-                                                                    (Prims.of_int (183))
+                                                                    (Prims.of_int (184))
                                                                     (Prims.of_int (39)))))
                                                                     (FStar_Sealed.seal
                                                                     (Obj.magic
                                                                     (FStar_Range.mk_range
                                                                     "Pulse.Checker.STApp.fst"
-                                                                    (Prims.of_int (180))
+                                                                    (Prims.of_int (181))
                                                                     (Prims.of_int (9))
-                                                                    (Prims.of_int (183))
+                                                                    (Prims.of_int (184))
                                                                     (Prims.of_int (39)))))
                                                                     (Obj.magic
                                                                     (FStar_Tactics_Effect.tac_bind
@@ -1583,17 +1618,17 @@ let (check :
                                                                     (Obj.magic
                                                                     (FStar_Range.mk_range
                                                                     "Pulse.Checker.STApp.fst"
-                                                                    (Prims.of_int (183))
+                                                                    (Prims.of_int (184))
                                                                     (Prims.of_int (16))
-                                                                    (Prims.of_int (183))
+                                                                    (Prims.of_int (184))
                                                                     (Prims.of_int (38)))))
                                                                     (FStar_Sealed.seal
                                                                     (Obj.magic
                                                                     (FStar_Range.mk_range
                                                                     "Pulse.Checker.STApp.fst"
-                                                                    (Prims.of_int (180))
+                                                                    (Prims.of_int (181))
                                                                     (Prims.of_int (31))
-                                                                    (Prims.of_int (183))
+                                                                    (Prims.of_int (184))
                                                                     (Prims.of_int (39)))))
                                                                     (Obj.magic
                                                                     (Pulse_Syntax_Printer.term_to_string
@@ -1608,17 +1643,17 @@ let (check :
                                                                     (Obj.magic
                                                                     (FStar_Range.mk_range
                                                                     "Pulse.Checker.STApp.fst"
-                                                                    (Prims.of_int (180))
+                                                                    (Prims.of_int (181))
                                                                     (Prims.of_int (31))
-                                                                    (Prims.of_int (183))
+                                                                    (Prims.of_int (184))
                                                                     (Prims.of_int (39)))))
                                                                     (FStar_Sealed.seal
                                                                     (Obj.magic
                                                                     (FStar_Range.mk_range
                                                                     "Pulse.Checker.STApp.fst"
-                                                                    (Prims.of_int (180))
+                                                                    (Prims.of_int (181))
                                                                     (Prims.of_int (31))
-                                                                    (Prims.of_int (183))
+                                                                    (Prims.of_int (184))
                                                                     (Prims.of_int (39)))))
                                                                     (Obj.magic
                                                                     (FStar_Tactics_Effect.tac_bind
@@ -1626,17 +1661,17 @@ let (check :
                                                                     (Obj.magic
                                                                     (FStar_Range.mk_range
                                                                     "Pulse.Checker.STApp.fst"
-                                                                    (Prims.of_int (182))
+                                                                    (Prims.of_int (183))
                                                                     (Prims.of_int (16))
-                                                                    (Prims.of_int (182))
+                                                                    (Prims.of_int (183))
                                                                     (Prims.of_int (39)))))
                                                                     (FStar_Sealed.seal
                                                                     (Obj.magic
                                                                     (FStar_Range.mk_range
                                                                     "Pulse.Checker.STApp.fst"
-                                                                    (Prims.of_int (180))
+                                                                    (Prims.of_int (181))
                                                                     (Prims.of_int (31))
-                                                                    (Prims.of_int (183))
+                                                                    (Prims.of_int (184))
                                                                     (Prims.of_int (39)))))
                                                                     (Obj.magic
                                                                     (Pulse_Syntax_Printer.term_to_string
@@ -1651,17 +1686,17 @@ let (check :
                                                                     (Obj.magic
                                                                     (FStar_Range.mk_range
                                                                     "Pulse.Checker.STApp.fst"
-                                                                    (Prims.of_int (180))
+                                                                    (Prims.of_int (181))
                                                                     (Prims.of_int (31))
-                                                                    (Prims.of_int (183))
+                                                                    (Prims.of_int (184))
                                                                     (Prims.of_int (39)))))
                                                                     (FStar_Sealed.seal
                                                                     (Obj.magic
                                                                     (FStar_Range.mk_range
                                                                     "Pulse.Checker.STApp.fst"
-                                                                    (Prims.of_int (180))
+                                                                    (Prims.of_int (181))
                                                                     (Prims.of_int (31))
-                                                                    (Prims.of_int (183))
+                                                                    (Prims.of_int (184))
                                                                     (Prims.of_int (39)))))
                                                                     (Obj.magic
                                                                     (FStar_Tactics_Effect.tac_bind
@@ -1669,9 +1704,9 @@ let (check :
                                                                     (Obj.magic
                                                                     (FStar_Range.mk_range
                                                                     "Pulse.Checker.STApp.fst"
-                                                                    (Prims.of_int (181))
+                                                                    (Prims.of_int (182))
                                                                     (Prims.of_int (16))
-                                                                    (Prims.of_int (181))
+                                                                    (Prims.of_int (182))
                                                                     (Prims.of_int (42)))))
                                                                     (FStar_Sealed.seal
                                                                     (Obj.magic
@@ -1743,17 +1778,17 @@ let (check :
                                                                     (Obj.magic
                                                                     (FStar_Range.mk_range
                                                                     "Pulse.Checker.STApp.fst"
-                                                                    (Prims.of_int (186))
+                                                                    (Prims.of_int (187))
                                                                     (Prims.of_int (31))
-                                                                    (Prims.of_int (186))
+                                                                    (Prims.of_int (187))
                                                                     (Prims.of_int (123)))))
                                                                     (FStar_Sealed.seal
                                                                     (Obj.magic
                                                                     (FStar_Range.mk_range
                                                                     "Pulse.Checker.STApp.fst"
-                                                                    (Prims.of_int (186))
+                                                                    (Prims.of_int (187))
                                                                     (Prims.of_int (9))
-                                                                    (Prims.of_int (186))
+                                                                    (Prims.of_int (187))
                                                                     (Prims.of_int (123)))))
                                                                     (Obj.magic
                                                                     (FStar_Tactics_Effect.tac_bind
@@ -1761,9 +1796,9 @@ let (check :
                                                                     (Obj.magic
                                                                     (FStar_Range.mk_range
                                                                     "Pulse.Checker.STApp.fst"
-                                                                    (Prims.of_int (186))
+                                                                    (Prims.of_int (187))
                                                                     (Prims.of_int (96))
-                                                                    (Prims.of_int (186))
+                                                                    (Prims.of_int (187))
                                                                     (Prims.of_int (122)))))
                                                                     (FStar_Sealed.seal
                                                                     (Obj.magic
